src/named/Compilers.v
@@ -1,1219 +1,554 @@
-
-Require Import mathcomp.ssreflect.all_ssreflect.
 Set Implicit Arguments.
-Unset Strict Implicit.
-Unset Printing Implicit Defensive.
 Set Bullet Behavior "Strict Subproofs".
 
-From Utils Require Import Utils BoolAsProp.
-From Named Require Import Exp ARule ImCore.
-Require Import String.
-
-(* TODO: this does not admit for optimization *)
-(* TODO! : trying to define compilation for to-be-inferred terms;
-   how do I include info from the type?
- *)
-Variant compiler_case : Set :=
-| sort_case : (* target *) sort -> compiler_case
-| term_case :  (* target *) exp -> compiler_case.
-
-Definition eq_compiler_case c1 c2 : bool :=
-  match c1,c2 with
-  | sort_case t1, sort_case t2 => (t1 == t2)
-  | term_case e1, term_case e2 => (e1 == e2)
-  | _,_ => false
-  end.
-
-Lemma eq_compiler_caseP c1 c2 : reflect (c1 = c2) (eq_compiler_case c1 c2).
-Proof using .
-  destruct c1; destruct c2; simpl;  solve_reflect_norec.
-Qed.
-
-Definition compiler_case_eqMixin := Equality.Mixin eq_compiler_caseP.
-
-Canonical compiler_case_eqType := @Equality.Pack compiler_case compiler_case_eqMixin.
-
-(* each element is the map for that constructor *)
-Definition compiler := named_list compiler_case.
-
-Section CompilesTo.
-  Context (src tgt : lang) (cmp : compiler).
-
-  Inductive term_compiles_to : ctx -> exp -> sort -> ctx -> exp -> sort -> Prop :=
-  | compile_var x c t
-    : (x,t) \in c ->
-      ctx_compiles_to c c' ->
-      (x,t') \in c' ->
-      term_compiles_to c (var x) t (var x)
-  | compile_con c n s e es es' c' args t
-    : (n, term_rule c' args t) \in src ->
-      (n, term_case e) \in cmp ->
-      (*Note: need to check wfness to get my hands on es *)
-      wf_args src c s args es c' ->
-      args_compile_to c es c' es' ->
-      term_compiles_to c (con n s) t[/with_names_from c' es/] e[/with_names_from c' es'/]
-  | compile_conv c e t t' e'
-    : term_compiles_to c e t e' -> le_sort src c t t' -> term_compiles_to c e t' e'
-  with args_compile_to : ctx -> list exp -> named_list sort -> list exp -> Prop :=
-  | compile_nil c : args_compile_to c [::] [::] [::]
-  | compile_cons c es c' es' e t e' n
-    : args_compile_to c es c' es' ->
-      term_compiles_to c e t[/with_names_from c' es/] e' ->
-      args_compile_to c (e::es) ((n,t)::c') (e'::es')
-  with sort_compiles_to : ctx -> sort -> sort -> Prop :=
-  | compile_scon c n s es es' c' args t
-    : (n, sort_rule c' args) \in src ->
-      (n, sort_case t) \in cmp ->
-      (*Note: need to check wfness to get my hands on es *)
-      wf_args src c s args es c' ->
-      args_compile_to c es c' es' ->
-      sort_compiles_to c (scon n s) t[/with_names_from c' es'/]
-  with ctx_compiles_to : ctx -> ctx -> Prop :=
-  | compile_ctx_nil : ctx_compiles_to [::] [::]
-  | compile_ctx_cons c c' t t' n
-    : ctx_compiles_to c c' ->
-      sort_compiles_to c t t' ->
-      fresh n c ->
-      ctx_compiles_to ((n,t)::c) ((n,t')::c').
-
-  Inductive 
-
-  Hint Constructors term_compiles_to args_compile_to sort_compiles_to ctx_compiles_to : imcore.
+Require Import List String.
+Import ListNotations.
+Open Scope string.
+Open Scope list.
+From Utils Require Import Utils.
+From Named Require Import Core.
+Import Exp.Notations.
 
 
-  Lemma term_compiles_is_wf c e t e'
-    : term_compiles_to c e t e' -> wf_term src c e t.
-  Proof.
-    induction 1; eauto with imcore.
-  Qed.
-  Hint Resolve term_compiles_is_wf : imcore.
+(* each element is the image for that constructor or axiom*)
+Variant compiler_case :=
+ | term_case (args : list string) (e:exp)
+ | sort_case (args : list string) (t:sort).
+Definition compiler := named_list compiler_case. 
 
-  (*TODO Go the other way; should rely on compiler wsness*)
-  Lemma term_wf_compiles c e t
-    : wf_term src c e t -> exists e', term_compiles_to c e t e'.
-  Proof.
-  Abort.
+Section CompileFn.
+  Context (tgt : lang)
+          (cmp : compiler)
+          (src : lang).
+
+  (* does not use src or tgt, only cmp *)
+  Fixpoint compile (e : exp) : exp :=
+    match e with
+    | var x => var x
+    | con n s =>
+      (*TODO: return Some and use default typeclass?*)
+      let default := con "ERR" [] in
+      let arg_terms := map compile s in
+      match named_list_lookup_err cmp n with
+      | Some (term_case args e) => e[/combine args arg_terms/]
+      | _ => default
+      end
+    end.
   
-  (*TODO: move to utils*)
-  Lemma subseq_nil {A:eqType} (l : list A) : subseq [::] l.
-  Proof.
-    destruct l; simpl; auto.
-  Qed.
-
-  Lemma args_compile_are_wf c s args es c' es'
-    : args_compile_to c es c' es' ->
-      size args = size s ->
-      subseq (zip args s) (with_names_from c' es) ->
-      wf_args src c s args es c'.
-  Proof.
-    intro acmp.
-    revert args s.
-    induction acmp; intros args s;
-      destruct args; destruct s; simpl;
-        let H := fresh in
-        intro H; inversion H; clear H;
-          let H := fresh in
-          intro H; inversion H; clear H; subst; auto with imcore.
-    {
-      constructor; eauto with imcore.
-      apply IHacmp; simpl; eauto with imcore.
-      apply subseq_nil.
-    }
-    {
-      move: H3 => /orP [ /andP [ /eqP ] |].
-      {
-        case; intros; subst; eauto with imcore.
-      }
-      {
-        intros.
-        constructor; eauto with imcore.
-        apply IHacmp; simpl; eauto.
-      }
-    }
-  Qed.
-  Hint Resolve args_compile_are_wf : imcore.
+  (* does not use src or tgt, only cmp *)
+  Definition compile_sort (t : sort) : sort :=
+    match t with
+    | scon n s =>
+      (*TODO: return Some and use default typeclass?*)
+      let default := scon "ERR" [] in
+      let arg_terms := map compile s in
+      match named_list_lookup_err cmp n with
+      | Some (sort_case args t) => t[/combine args arg_terms/]
+      | _ => default
+      end
+    end.  
   
-  Lemma sort_compiles_is_wf c t t'
-    : sort_compiles_to c t t' -> wf_sort src c t.
-  Proof.
-    destruct 1; eauto with imcore.
-  Qed.
-  Hint Resolve sort_compiles_is_wf : imcore.
+  Definition compile_args := map compile.
 
-  (* First we specify the properties semantically,
+  Definition compile_subst (s : named_list exp) := named_map compile s.
+
+  Definition compile_ctx (c:named_list sort) := named_map compile_sort c.
+
+   (* First we specify the properties semantically,
      then inductively on the compiler. TODO: prove equivalent
    *)
   Definition sort_wf_preserving_sem :=
-    forall c c' t t', ctx_compiles_to c c' -> 
-                      sort_compiles_to c t t' -> 
-                      wf_sort tgt c' t'.
+    forall c t, wf_sort src c t ->
+                wf_sort tgt (compile_ctx c) (compile_sort t).
 
   Definition term_wf_preserving_sem :=
-    forall c c' e e' t t', ctx_compiles_to c c' -> 
-                           sort_compiles_to c t t' -> 
-                           term_compiles_to c e t e' -> 
-                           wf_term tgt c' e' t'.
+    forall c e t,
+      wf_term src c e t ->
+      wf_term tgt (compile_ctx c) (compile e) (compile_sort t).
 
-  Definition sort_le_preserving_sem :=
-    forall c c' t1 t2 t1' t2',
-      ctx_compiles_to c c' -> 
-      sort_compiles_to c t1 t1' -> 
-      sort_compiles_to c t2 t2' -> 
-      le_sort src c t1 t2 ->
-      le_sort tgt c' t1' t2'.
-
-  Definition term_le_preserving_sem :=
-    forall c c' e1 e2  e1' e2' t t',
-      ctx_compiles_to c c' -> 
-      sort_compiles_to c t t' -> 
-      term_compiles_to c e1 t e1' -> 
-      term_compiles_to c e2 t e2' ->
-      le_term src c t e1 e2 ->
-      le_term tgt c' t' e1' e2'.
+  Definition sort_eq_preserving_sem :=
+    forall c t1 t2,
+      eq_sort src c t1 t2 ->
+      eq_sort tgt (compile_ctx c) (compile_sort t1) (compile_sort t2).
+  
+  Definition term_eq_preserving_sem :=
+    forall c t e1 e2,
+      eq_term src c t e1 e2 ->
+      eq_term tgt (compile_ctx c) (compile_sort t) (compile e1) (compile e2).
 
   Definition args_wf_preserving_sem :=
-    forall c c' s' args es es' c2 c2',
-      ctx_compiles_to c c' ->
-      args_compile_to c es c2 es' ->
-      ctx_compiles_to c2 c2' ->
-      size args = size s' ->
-      subseq (zip args s') (with_names_from c2' es') ->
-      wf_args tgt c' s' args es' c2'.
+    forall c s c',
+      wf_args src c s c' ->
+      wf_args tgt (compile_ctx c) (compile_args s) (compile_ctx c').
 
-
-  Definition args_le_preserving_sem :=
-    forall c c' s1' s2' args es1 es2 es1' es2' c2 c2',
-      ctx_compiles_to c c' ->
-      args_compile_to c es1 c2 es1' ->
-      args_compile_to c es2 c2 es2' ->
-      ctx_compiles_to c2 c2' ->
-      size args = size s1' ->
-      subseq (zip args s1') (with_names_from c2' es1') ->
-      size args = size s2' ->
-      subseq (zip args s2') (with_names_from c2' es2') ->
-      le_args tgt c' c2' s1' s2' args es1' es2'.
-
+  Definition subst_eq_preserving_sem :=
+    forall c c' s1 s2,
+      eq_subst src c c' s1 s2 ->
+      eq_subst tgt (compile_ctx c) (compile_ctx c') (compile_subst s1) (compile_subst s2).
+   
   Definition ctx_wf_preserving_sem :=
-    forall c c',
-      ctx_compiles_to c c' ->
-      wf_ctx tgt c'.
+    forall c, wf_ctx src c -> wf_ctx tgt (compile_ctx c).
 
+  (*Set up to match the combined scheme for the judgment inductives *)
   Definition semantics_preserving :=
-    sort_wf_preserving_sem /\ term_wf_preserving_sem /\ args_wf_preserving_sem
-    /\ sort_le_preserving_sem /\ term_le_preserving_sem /\ args_le_preserving_sem.
+    sort_eq_preserving_sem /\ term_eq_preserving_sem /\ subst_eq_preserving_sem
+    /\ sort_wf_preserving_sem /\ term_wf_preserving_sem /\ args_wf_preserving_sem
+    /\ ctx_wf_preserving_sem.
 
+End CompileFn.
 
-  Lemma ctx_compiles_fst c c' : ctx_compiles_to c c' -> map fst c = map fst c'.
-  Proof.
-    induction 1; simpl; congruence.
-  Qed.
-      
-  Lemma fresh_compile_ctx c c' n
-    : fresh n c -> ctx_compiles_to c c' -> fresh n c'.
-  Proof using.
-    unfold fresh; intros; erewrite <- ctx_compiles_fst; eauto.
-  Qed.
-  
-End CompilesTo.
-#[export] Hint Constructors term_compiles_to args_compile_to sort_compiles_to ctx_compiles_to : imcore.
-#[export] Hint Resolve term_compiles_is_wf : imcore.
-#[export] Hint Resolve args_compile_are_wf : imcore.
-#[export] Hint Resolve sort_compiles_is_wf : imcore.
-#[export] Hint Resolve fresh_compile_ctx : imcore.
+(*
+First we define an inductively provable (and in fact decidable) property 
+of elaborated compilers.
+*)
 
-  
 (*TODO: this is an equal or stronger property (which?); includes le principles;
   formalize the relationship to those above and le semantic statements *)
-(*TODO: since things aren't functions, there are quantifier issues;
-  these may need some adjustment
- *)
-Inductive preserving_compiler (target : lang) : lang -> compiler -> Prop :=
-| preserving_compiler_nil : preserving_compiler target [::] [::]
-| preserving_compiler_sort : forall src cmp n c args t,
-    preserving_compiler target src cmp ->
-    (forall c',
-        (* Notable: only uses the previous parts of the compiler on c *)
-        ctx_compiles_to src cmp c c' ->
-        wf_sort target c' t) ->
-    preserving_compiler target ((n,sort_rule c args) :: src) ((n, sort_case t)::cmp)
-| preserving_compiler_term : forall src cmp n c args t e,
-    preserving_compiler target src cmp ->
-    (forall c' t',
-        (* Notable: only uses the previous parts of the compiler on c,t *)
-        ctx_compiles_to src cmp c c' ->
-        sort_compiles_to src cmp c t t' ->
-        wf_term target c' e t') ->
-    preserving_compiler target ((n,term_rule c args t) :: src) ((n, term_case e)::cmp)
-| preserving_compiler_sort_le : forall src cmp n c args t1 t2,
-    preserving_compiler target src cmp ->
-    (forall c' t1' t2',
-        (* Notable: only uses the previous parts of the compiler on c,t1, t2 *)
-        ctx_compiles_to src cmp c c' ->
-        sort_compiles_to src cmp c t1 t1' ->
-        sort_compiles_to src cmp c t2 t2' ->
-        le_sort src c t1 t2 ->
-        le_sort target c' t1' t2') ->
-    preserving_compiler target ((n,sort_rule c args) :: src) cmp
-| preserving_compiler_term_le : forall src cmp n c args t e1 e2,
-    preserving_compiler target src cmp ->
-    (forall c' t' e1' e2',
-        (* Notable: only uses the previous parts of the compiler on c,t1, t2 *)
-        ctx_compiles_to src cmp c c' ->
-        sort_compiles_to src cmp c t t' ->
-        term_compiles_to src cmp c e1 t e1' ->
-        term_compiles_to src cmp c e2 t e2' ->
-        le_term src c t e1 e2 ->
-        le_term target c' t' e1' e2') ->
-    preserving_compiler target ((n,sort_rule c args) :: src) cmp.
-Hint Constructors preserving_compiler : imcore.
+Inductive preserving_compiler (target : lang) : compiler -> lang -> Prop :=
+| preserving_compiler_nil : preserving_compiler target [] []
+| preserving_compiler_sort : forall cmp l n c args t,
+    preserving_compiler target cmp l ->
+    (* Notable: only uses the previous parts of the compiler on c *)
+    wf_sort target (compile_ctx cmp c) t ->
+    preserving_compiler target ((n,sort_case (map fst c) t)::cmp) ((n,sort_rule c args) :: l)
+| preserving_compiler_term : forall cmp l n c args e t,
+    preserving_compiler target cmp l ->
+    (* Notable: only uses the previous parts of the compiler on c, t *)
+    wf_term target (compile_ctx cmp c) e (compile_sort cmp t) ->
+    preserving_compiler target ((n, term_case (map fst c) e)::cmp) ((n,term_rule c args t) :: l)
+| preserving_compiler_sort_eq : forall cmp l n c t1 t2,
+    preserving_compiler target cmp l ->
+    (* Notable: only uses the previous parts of the compiler on c *)
+    eq_sort target (compile_ctx cmp c) (compile_sort cmp t1) (compile_sort cmp t2) ->
+    preserving_compiler target cmp ((n,sort_eq_rule c t1 t2) :: l)
+| preserving_compiler_term_eq : forall cmp l n c e1 e2 t,
+    preserving_compiler target cmp l ->
+    (* Notable: only uses the previous parts of the compiler on c *)
+    eq_term target (compile_ctx cmp c) (compile_sort cmp t) (compile cmp e1) (compile cmp e2) ->
+    preserving_compiler target cmp ((n,term_eq_rule c e1 e2 t) :: l).
 
 
-
-Lemma wf_empty_sort c t : ~wf_sort [::] c t.
-Proof using .
-  by inversion.
-Qed.
-
-Lemma wf_empty_ctx c : wf_ctx [::] c -> c = [::].
-Proof using .
-  case; auto.
-  intros.
-  exfalso.
-  eapply wf_empty_sort; eassumption.
-Qed.
-
-(*
-Lemma wf_empty_term c e t : wf_ctx [::] c -> ~wf_term [::] c e t.
-Proof using .
-  intros wfc wft.
-  elim: wft wfc; eauto.
-  intros n t0 nin.
-  move /wf_empty_ctx => wfe.
-  move: wfe nin => ->.
-  auto.  
-Qed.
-*)
-
-(*TODO: move to core*)
-
-Lemma with_names_from_nil_r (c : ctx) : with_names_from c (@nil exp) = [::].
+Lemma fresh_compile_ctx x cmp c
+  : fresh x c -> fresh x (compile_ctx cmp c).
 Proof.
-  case: c; simpl; auto; case; auto.
+  induction c; basic_goal_prep;
+    pre_rewrite_core_crush.
 Qed.
+Hint Resolve fresh_compile_ctx : lang_core.
 
 
+Lemma all_fresh_compile_ctx cmp c
+  : all_fresh c -> all_fresh (compile_ctx cmp c).
+Proof.
+  induction c; basic_goal_prep;
+    pre_rewrite_core_crush.
+Qed.
+Hint Resolve all_fresh_compile_ctx : pfcore.
 
-Ltac f_equal_match :=
+
+Lemma compile_strengthen_term src tgt cmp c e t n cc
+  : wf_term src c e t ->
+    preserving_compiler tgt cmp src ->
+    fresh n cmp ->
+    compile ((n,cc)::cmp) e = compile cmp e.
+Admitted.
+
+Lemma compile_strengthen_sort src tgt cmp c t n cc
+  : wf_sort src c t ->
+    preserving_compiler tgt cmp src ->
+    fresh n cmp ->
+    compile_sort ((n,cc)::cmp) t = compile_sort cmp t.
+Admitted.
+
+Lemma compile_strengthen_ctx src tgt cmp c n cc
+  : wf_ctx src c ->
+    preserving_compiler tgt cmp src ->
+    fresh n cmp ->
+    compile_ctx ((n,cc)::cmp) c = compile_ctx cmp c.
+Admitted.
+
+
+Lemma fresh_lang_fresh_cmp lt cmp l n
+  : preserving_compiler lt cmp l ->
+    fresh n l -> fresh n cmp.
+Proof.
+  induction 1; basic_goal_prep;
+    pre_rewrite_core_crush.
+Qed.
+Hint Resolve fresh_lang_fresh_cmp : lang_core.
+
+Ltac rewrite_strengthen :=
   match goal with
-  | [|- match ?e with _ => _ end = match ?e with _ => _ end]
-    => let e':= fresh in remember e as e'; destruct e'
+  | [H : wf_ctx _ _, pr : preserving_compiler _ _ _ |-_] =>
+    rewrite (compile_strengthen_ctx _ H pr); eauto with pfcore
+  | [H : wf_sort _ _ _, pr : preserving_compiler _ _ _ |-_] =>
+    rewrite (compile_strengthen_sort _ H pr); eauto with pfcore
+  | [H : wf_term _ _ _ _, pr : preserving_compiler _ _ _ |-_] =>
+    rewrite (compile_strengthen_term _ H pr); eauto with pfcore
   end.
 
-(*
-Lemma lookup_in_tail c c' n t s s'
-    : let cs' := with_names_from (c'++ c) (s' ++ s) in
-    size s == size c ->
-    size s' == size c' ->
-    all_fresh (c' ++ c) ->
-    (n,t) \in c ->
-              named_list_lookup (var n) cs' n =
-              named_list_lookup (var n) (with_names_from c s) n.
-Proof.
-  simpl.
-  elim: c' s'.
-  {
-    case; simpl; auto.
-    intros a l _.
-    move /eqP; inversion.
-  }
-  {
-    intros until s'.
-    case: s'.
-    {
-      intro b.
-      move /eqP; inversion.
-    }
-    {
-      destruct a.
-      intros e s' szeq.
-      simpl; move /eqP; case; move /eqP => szeq'.
-      move /andP => [fs0 nlaf] nin.
-      suff: ((n=?s0)%string = false); [move ->; eauto|].
-      admit.
-    }
-  }
-Admitted.
+(* TODO: work on
+Ltac inductive_implies_semantic_rule :=
+intros wfl pr wfl';
+  revert wfl'; induction pr; simpl; [easy|..];
+    repeat (simpl; autorewrite with bool_utils pfcore utils);
+    intuition; subst;
+      try match goal with
+          | [wfl : wf_lang ?l, H: is_true((_,_) \in ?l)|-_] =>
+            let H':= fresh in pose proof (rule_in_wf wfl H) as H'; safe_invert H'
+          end;
+      repeat rewrite_strengthen; [];
+  cbn [compile_pf]; 
+    repeat (simpl; autorewrite with bool_utils pfcore utils);
+  assumption.
 *)
-
-(*
-Local Ltac in_preserving_sort_rec :=
-  intros;
-      match goal with
-        [ Hin : is_true(_\in_),
-          IH : is_true(_\in_) -> exists t,_ |- _] =>
-        move: (IH Hin); case; intros
-      end; solve [eauto 3 | eexists; rewrite in_cons; apply /orP; eauto].
-
-Lemma in_preserving_sort lt ls cmp n c' args
-  : preserving_compiler lt ls cmp ->
-    (n, sort_rule c' args) \in ls ->
-    exists t,(n, sort_case t) \in cmp.
-Proof using .
-  elim; simpl; eauto; intros;
-    try  match goal with
-    [ H : is_true(_\in_::_)|- _] =>
-    revert H; rewrite in_cons; move /orP; case
-    end; try solve [move/eqP; case; done| in_preserving_sort_rec].
-  { 
-    move /eqP => [neq ceq].
-    subst.
-    exists t.
-    rewrite in_cons.
-    apply /orP.
-    left.
-    apply /eqP; reflexivity.
-  }
-  Unshelve.
-  exact (scon "ERR" [::]).
-Qed.
-
-Lemma in_preserving_term lt cmp ls n c' args t
-  : preserving_compiler lt cmp ls ->
-    (n, term_rule c' args t) \in ls ->
-    exists e,(n, term_case (map fst c') e) \in cmp.
-Proof using .
-  elim; simpl; eauto; intros;
-    try  match goal with
-    [ H : is_true(_\in_::_)|- _] =>
-    revert H; rewrite in_cons; move /orP; case
-    end; try solve [move/eqP; case; done| in_preserving_sort_rec].
-  { 
-    move /eqP => [neq ceq teq].
-    subst.
-    exists e.
-    rewrite in_cons.
-    apply /orP.
-    left.
-    apply /eqP; reflexivity.
-  }
-  Unshelve.
-  exact (con "ERR" [::]).
-Qed.
- *)
-
-(*
-(*TODO: use existing lemmas*)
-Lemma named_list_all_fresh_lookup {A : eqType} l n (e default : A)
-  : all_fresh l ->
-    (n, e) \in l ->
-    named_list_lookup default l n = e.
-Proof using .
-  elim: l; [ by cbv |].
-  move => [n' e'] l IH; simpl.
-  move /andP => [ fn allf].
-  rewrite in_cons.
-  case neq: (n == n').
-  case eeq: (e == e').
-  {
-    move: neq eeq => /eqP neq /eqP eeq.
-    rewrite -!neq -!eeq.
-    move /orP; case; intros; subst;
-    rewrite eqb_refl; reflexivity.
-  }
-  {
-    pose neq' := neq.
-    cbn.
-    cbn in neq.
-    rewrite neq.
-    rewrite eeq.
-    simpl.
-    clear IH.
-    move: neq' fn => /eqP ->.
-    intros.
-    exfalso.
-    pose p := (fresh_neq_in fn H).
-    move: p.
-    move /eqP.
-    done.
-  }
-  {
-    suff: ((n, e) == (n', e') = false); [ move ->; simpl|].
-    2:{
-      rewrite -Bool.negb_true_iff.
-      apply /negP.
-      move /eqP.
-      case.
-      move /eqP.
-      by rewrite neq.
-    }
-    pose p := neq; cbn in p; rewrite p; clear p.
-    auto.
-  } 
-Qed.
-*)
-
-Lemma preserving_compiler_fresh n lt ls cmp
-  : preserving_compiler lt ls cmp ->
-    fresh n ls ->
-    fresh n cmp.
-Proof using .
-  unfold fresh; induction 1; simpl; auto;
-    rewrite !in_cons.
-  (*
-  all: move /negP; intros H'.
-  all: apply /negP; move /orP; intro H''.
-  all: apply H'; clear H'; try apply /orP.
-  all: intuition; try right; eauto.
-  rewrite H1 in IHpreserving_compiler.*)
-Admitted.
-Hint Resolve  preserving_compiler_fresh : imcore.
   
-Lemma preserving_compiler_all_fresh lt cmp ls
-  : preserving_compiler lt ls cmp ->
-    all_fresh ls ->
-    all_fresh cmp.
-Proof using .
-  induction 1; simpl; auto.
-  (*TODO: bool to prop utility*)
-Admitted.
-Hint Resolve preserving_compiler_all_fresh : judgment.
 
-(* TODO: move to Core *)
-Lemma wf_lang_all_fresh l : wf_lang l -> all_fresh l.
+Lemma inductive_implies_semantic_sort_axiom ls lt cmp name c t1 t2
+  : wf_lang lt -> preserving_compiler lt cmp ls -> wf_lang ls ->
+    In (name, sort_eq_rule c t1 t2) ls ->
+    eq_sort lt (compile_ctx cmp c) (compile_sort cmp t1) (compile_sort cmp t2).
 Proof.
-  elim; intros; simpl in *; auto.
-  apply /andP; auto.
+  induction 2; basic_goal_prep; 
+    pre_rewrite_core_crush.
+  
 Qed.
-Hint Resolve wf_lang_all_fresh : judgment.
 
-(*
-Lemma term_fresh_strengthen n cc l cmp c e t
-  : fresh n l ->
-    wf_term l c e t ->
-    compile_term ((n, cc) :: cmp) e = compile_term cmp e
-with args_fresh_strengthen n cc l cmp c s args es c'
-  : fresh n l ->
-    wf_args l c s args es c' ->
-    compile_args ((n, cc) :: cmp) s = compile_args cmp s.
-Proof using .
-  {
-    intro_to wf_term; inversion; subst; simpl in *; eauto.
-    {
-      suff: ((n0 =? n)%string = false);[ move ->|].
-      {
-        f_equal_match; auto.
-        change (map (compile_term ?cmp)) with (compile_args cmp).
-        erewrite args_fresh_strengthen; eauto.
-      }
-      {
-        apply /negP.
-        apply /negP.
-        eapply fresh_neq_in; eauto.
-      }
-    }
-  }
-  {
-    intro_to wf_args; inversion; subst; simpl in *; eauto.
-    f_equal; eauto.
-  }    
-Qed.    
+
+Lemma inductive_implies_semantic_term_axiom ls lt cmp name c e1 e2 t
+  : wf_lang lt -> preserving_compiler lt cmp ls -> wf_lang ls ->
+    (name, wf_term_eq c e1 e2 t) \in ls ->
+    eq_term lt (compile_ctx cmp c) (compile_pf cmp (ax name))
+            (compile cmp t) (compile cmp e1) (compile cmp e2).
+Proof.
+  inductive_implies_semantic_rule.
+Qed.
+
+
+(*TODO: move to utils*)
+Lemma with_names_from_map_is_named_map (A B C:Set) (f : A -> B) (l1 : named_list C) l2
+  : with_names_from l1 (map f l2) = named_map f (with_names_from l1 l2).
+Proof.
+  revert l2; induction l1;
+    destruct l2; break; subst; simpl; f_equal; eauto.
+Qed.
+(* TODO: do I want to rewrite like this?
+  Hint Rewrite with_names_from_map_is_named_map : utils.*)
+
+
+Lemma with_names_from_compile_ctx (A:Set) cmp c (s : list A)
+  : with_names_from (compile_ctx cmp c) s
+    = with_names_from c s.
+Proof.
+  revert s; induction c;
+    destruct s; break; pfcore_crush.
+  f_equal; pfcore_crush.
+Qed.
+  
+Lemma wf_subst_from_wf_args l c s c'
+  : wf_args l c s c' ->
+    wf_subst l c (with_names_from c' s) c'.
+Proof.
+  induction 1; pfcore_crush.
+Qed.
+Hint Resolve wf_subst_from_wf_args : pfcore.
     
-Lemma sort_fresh_strengthen n cc l cmp c t
-  : fresh n l ->
-    wf_sort l c t ->
-    compile_sort ((n, cc) :: cmp) t = compile_sort cmp t.
-Proof using .
-  intro_to wf_sort; inversion; subst.
-  simpl.
-  suff: ((n0 =? n)%string = false);[ move ->|].
-  {
-    f_equal_match; auto.
-    erewrite args_fresh_strengthen; eauto.
-  }
-  {
-    apply /negP.
-    apply /negP.
-    eapply fresh_neq_in; eauto.
-  }
-Qed.
-  
-Lemma ctx_fresh_strengthen n cc l cmp c
-  : fresh n l ->
-    wf_ctx l c ->
-    compile_ctx ((n, cc) :: cmp) c = compile_ctx cmp c.
+Definition id_args {A} (c : named_list A) : list wfexp :=
+  map wf_var (map fst c).
+
+
+Lemma compile_id_args A cmp (c : named_list A)
+  : map (compile cmp) (id_args c) = id_args c.
 Proof.
-  elim: c; simpl; auto.
-  intro_to wf_ctx; inversion; subst.
-  simpl.
-  f_equal; auto.
-  erewrite sort_fresh_strengthen; eauto.
+  unfold id_args.
+  induction c; break; simpl; f_equal; pfcore_crush.
+Qed.
+Hint Rewrite compile_id_args : pfcore.
+
+Lemma fst_equal_id_args_equal A B (c1 : named_list A) (c2 : named_list B)
+  : map fst c1 = map fst c2 -> id_args c1 = id_args c2.
+Proof.
+  unfold id_args; move => ->; reflexivity.
+Qed.
+
+Lemma compile_ctx_fst_equal cmp c
+  : map fst (compile_ctx cmp c) = map fst c.
+Proof.
+  induction c; break; simpl; f_equal; auto.
+Qed.
+
+Lemma id_args_wf l c
+  : wf_args l c (id_args c) c.
+Proof.
+Admitted.
+Hint Resolve id_args_wf : pfcore.
+
+
+Lemma zip_map_fst_is_with_names_from (A B : Set) (c : named_list A) (s : list B)
+  : zip (map fst c) s = with_names_from c s.
+Proof.
+  revert s; induction c; destruct s; break; cbn; pfcore_crush.
+Qed.
+Hint Rewrite zip_map_fst_is_with_names_from : utils.
+
+Lemma inductive_implies_semantic_sort_rule_id ls lt cmp name c args
+  : wf_lang lt -> preserving_compiler lt cmp ls -> wf_lang ls ->
+    (name, Pf.wf_sort_rule c args) \in ls ->
+    wf_sort lt (compile_ctx cmp c) (compile cmp (wf_con name (id_args c))).
+Proof.
+  intros wfl pr wfl';
+    revert wfl'; induction pr; simpl; [easy|..].
+  all: pfcore_crush.
+  {
+    safe_invert H0; pfcore_crush.      
+    cbn; pfcore_crush.
+    eapply wf_sort_subst_monotonicity; pfcore_crush.
+    erewrite with_names_from_names_eq.
+    apply wf_subst_from_wf_args.
+    repeat rewrite_strengthen.
+    erewrite fst_equal_id_args_equal; pfcore_crush.
+    by rewrite compile_ctx_fst_equal.
+    by rewrite compile_ctx_fst_equal.
+  }
+  {
+    cbn.
+    my_case Hn (name =? n)%string; pfcore_crush.
+    {
+      (*TODO: automate in boolutils *)
+      move: Hn => /eqP Hn; subst.
+      exfalso.
+      (*TODO: add modified lemma as hint*)
+      pose proof (fresh_neq_in H4 H0).
+      pfcore_crush.
+    }
+    case_match; pfcore_crush.
+      
+    eauto with pfcore.
+    case_match.
+    simpl in *.
+  
+  all: try solve [assert (wf_sort l c (wf_con name (id_args c))) by pfcore_crush;
+                  repeat rewrite_strengthen].
+  inversion H5.
+  inversion H5.
+  inversion H6.
+Qed.
+
+Lemma wf_con_id_args_subst (A:Set) name (c' : named_list A) s
+  : size c' = size s -> (wfexp_subst (with_names_from c' s) (wf_con name (id_args c'))) = (wf_con name s).
+Proof.
+  intros ?.
+  simpl; f_equal.
+  unfold id_args.
+Admitted.
+
+Lemma compile_named_list_lookup ls cmp s n
+  : compile ls cmp (named_list_lookup (wf_var n) s n)
+  = named_list_lookup (wf_var n) (compile_subst ls cmp s) n.
+Proof.
+  induction s; break; 
+    repeat (simpl; autorewrite with bool_utils pfcore utils); eauto with pfcore.
+  case_match; 
+    repeat (simpl; autorewrite with bool_utils pfcore utils); eauto with pfcore.
+Qed.
+
+Lemma compile_wfexp_subst ls cmp s e
+  : (compile ls cmp (wfexp_subst s e))
+    = wfexp_subst (compile_subst ls cmp s) (compile ls cmp e).
+Proof.
+  induction e; cbn.
+  {
+    apply compile_named_list_lookup.
+  }
+Admitted.
+Hint Rewrite compile_wfexp_subst : pfcore.
+
+Lemma compile_subst_with_names_from (A:Set) ls cmp (c':named_list A) s
+  : (compile_subst ls cmp (with_names_from c' s)) = with_names_from c' (map (compile ls cmp) s).
+Proof.
+  unfold compile_subst.
+  rewrite <- with_names_from_map_is_named_map.
+  reflexivity.
+Qed.
+
+Lemma id_subst_id (A:Set) (c' : named_list A) e
+  : wfexp_subst (with_names_from c' (id_args c')) e = e.
+Proof.
+Admitted.
+
+Lemma id_subst_id_args (A:Set) (c' : named_list A) s
+  : map (wfexp_subst (with_names_from c' (id_args c'))) s = s.
+Proof.
+  induction s; simpl; pfcore_crush; rewrite id_subst_id; pfcore_crush.
+Qed.
+
+
+Lemma compile_wfcon_sort ls cmp c' args s name t
+  : all_fresh ls ->
+    all_fresh cmp ->
+    (name, Pf.wf_sort_rule c' args) \in ls ->
+    (name, con_case t) \in cmp ->
+    (compile ls cmp (wf_con name s)) = wfexp_subst (with_names_from c' (compile_args ls cmp s)) t.
+Proof.
+  intros.
+  cbn.
+  case_match.
+  
+  
+Lemma inductive_implies_semantic_sort_rule ls lt cmp name c c' args s
+  : wf_lang lt -> preserving_compiler lt cmp ls -> wf_lang ls ->
+    (name, Pf.wf_sort_rule c' args) \in ls ->
+    (*wf_args ls c s c' ->*)
+    wf_args lt (compile_ctx ls cmp c) (compile_args ls cmp s) (compile_ctx ls cmp c') ->
+    wf_sort lt (compile_ctx ls cmp c) (compile ls cmp (wf_con name s)).
+Proof.
+  intros.
+  replace (wf_con name s) with (wfexp_subst (with_names_from c' s) (wf_con name (id_args c'))).
+  erewrite <- wf_con_id_args_subst.
+  rewrite compile_wfexp_subst.
+  eapply wf_sort_subst_monotonicity; pfcore_crush.
+  {
+    erewrite id_subst_id_args.
+               cbn; pfcore_crush.
+    pfcore_crush.
+  2:{
+    rewrite compile_subst_with_names_from.
+    erewrite with_names_from_names_eq.
+    eapply wf_subst_from_wf_args; pfcore_crush.
+    unfold compile_ctx; rewrite named_map_fst_eq.
+    reflexivity.
+  }
+  
+.
+    
+  TODO: need the right rewrites
+  eapply inductive_implies_semantic_sort_rule_id
+  
+  
+  intros wfl pr wfl';
+    revert wfl'; induction pr; simpl; [easy|..].
+  all: pfcore_crush.
+  {    
+    safe_invert H0; pfcore_crush.      
+    cbn; pfcore_crush.
+    erewrite <- with_names_from_compile_ctx.
+    eapply wf_sort_subst_monotonicity; pfcore_crush.
+    apply wf_subst_from_wf_args.
+    replace (compile_ctx l cmp c0)
+      with (compile_ctx ((n, Pf.wf_sort_rule c0 args0) :: l) ((n, con_case t) :: cmp) c0);
+      auto.
+    erewrite compile_strengthen_ctx; pfcore_crush.
+  }
+  {
+    (*Note: name != n*)
+    TODO: issue is that substitution s can use n
+                                                  
+                                                    
+    assert (wf_sort l c0 (wf_con name s)).
+    rewrite_strengthen.
+    
+    
+Fail Admitted.
+(*  
+  
+  all: repeat (simpl; autorewrite with bool_utils pfcore utils);
+    intuition; subst;
+      try match goal with
+          | [wfl : wf_lang ?l, H: is_true((_,_) \in ?l)|-_] =>
+            let H':= fresh in pose proof (rule_in_wf wfl H) as H'; safe_invert H'
+          end.
+  all: repeat rewrite_strengthen.
+  
+  (* TODO: need subst monotonicity *)
+
+  all: repeat (simpl; autorewrite with bool_utils pfcore utils);
+    intuition; subst;
+      try match goal with
+          | [wfl : wf_lang ?l, H: is_true((_,_) \in ?l)|-_] =>
+            let H':= fresh in pose proof (rule_in_wf wfl H) as H'; safe_invert H'
+          end.
+2:{  assert (name == 
+all: repeat rewrite_strengthen.
+{
+  cbn [compile]; 
+    repeat (simpl; autorewrite with bool_utils pfcore utils).
+  
+  assumption.
+  inductive_implies_semantic_rule.
+Qed.*)
+
+(*TODO: will this arrangement be useful?
+Lemma named_list_lookup_err_in_some {A:eqType} l x (v:A)
+  : all_fresh l -> ((x, v) \in l) -> named_list_lookup_err l x = Some v.
+Proof.
+  intros ?.
+  rewrite <- named_list_lookup_err_inb;
+    autorewrite with bool_utils; auto.
 Qed.  *)
 
 
-(*TODO:move to Core*)
-(* TODO:add hints?
-(* a hint for a common case*)
-Lemma wf_ctx_from_sort_rule_in l c n
-  : wf_lang l -> (n, sort_rule c) \in l -> wf_ctx l c.
+Lemma term_eq_in_lang_proof_in_compiler name lt cmp ls c e1 e2 t
+  : preserving_compiler lt cmp ls ->
+    (name, wf_term_eq c e1 e2 t) \in ls ->
+    exists p, (name, ax_case p) \in cmp.
 Proof.
-  intros wfl cin; apply rule_in_wf in cin; inversion cin; done.
-Qed.
-Hint Resolve wf_ctx_from_sort_rule_in : judgment.
-(* a hint for a common case*)
-Lemma wf_ctx_from_term_rule_in l c t n
-  : wf_lang l -> (n, term_rule c t) \in l -> wf_ctx l c.
-Proof.
-  intros wfl cin; apply rule_in_wf in cin; inversion cin; done.
-Qed.
-Hint Resolve wf_ctx_from_term_rule_in : judgment.
-(* a hint for a common case*)
-Lemma wf_sort_from_term_rule_in l c t n
-  : wf_lang l -> (n, term_rule c t) \in l -> wf_sort l c t.
-Proof.
-  intros wfl cin; apply rule_in_wf in cin; inversion cin; done.
-Qed.
-Hint Resolve wf_sort_from_term_rule_in : judgment.
-*)
-
-
-
-Local Ltac setup_inv_lem :=
-  let pc := fresh "pc" in
-  let wfl := fresh "wfl" in
-  let frls := fresh "frls" in
-  let frcmp := fresh "frcmp" in
-  intros pc wfl;
-  suff: all_fresh ls; eauto with judgment;  intro frls;
-  suff: all_fresh cmp; eauto with judgment; intro frcmp;
-  rewrite !all_fresh_in_once; auto;
-  revert pc wfl frls frcmp.
-
-(*
-(* TODO: relate independent judgment to elab
-   to port core lemmas.
-*)
-Parameter rule_in_wf
-     : forall (l : lang) (r : rule) (n : string),
-       wf_lang l -> (n, r) \in l -> wf_rule l r.
-
-Local Ltac inv_lem_step :=
-  match goal with
-  | H : wf_lang (_::_)|-_=> inversion H; subst; clear H
-  | H : wf_rule _ _|-_=>inversion H; subst; clear H
-  | H : is_true(_ || _) |- _=> move: H => /orP; case => H; break
-  | H : is_true(_ == _) |- _=> move: H => /eqP; (try by inversion); repeat case; intros; subst
-  | H : is_true(?a != ?a) |- _=> by rewrite eq_refl in H
-  | H : is_true(in_once _ _ _) |- wf_ctx _ _ =>
-    rewrite -all_fresh_in_once in H; auto; apply rule_in_wf in H; inversion H; subst; eassumption
-  | H : is_true(in_once _ _ _) |- wf_sort _ _ _ =>
-    rewrite -all_fresh_in_once in H; auto; apply rule_in_wf in H; inversion H; subst; eassumption
-  | H : is_true(in_once _ _ _) |- wf_term _ _ _ _ =>
-    rewrite -all_fresh_in_once in H; auto; apply rule_in_wf in H; inversion H; subst; eassumption
-  | |- context[ compile_ctx (_::_) _] => erewrite ctx_fresh_strengthen; eauto with judgment
-  | |- context[ compile_sort (_::_) _] => erewrite sort_fresh_strengthen; eauto with judgment
-  | |- context[ compile_term (_::_) _] => erewrite term_fresh_strengthen; eauto with judgment
-  end.
-*)
-
-(*
-Local Ltac prove_inv_lem :=
-  setup_inv_lem;
-  elim; [by cbv|..];
-    intros; simpl in *; break;
-  repeat inv_lem_step; eauto.
-*)
-
-Lemma invert_sort_case_eq t t0
-  : sort_case t = sort_case t0 <-> t = t0.
-Proof. intuition; inversion H; eauto with imcore. Qed.
-Hint Rewrite invert_sort_case_eq : imcore.
-
-Lemma invert_term_case_eq t t0
-  : term_case t = term_case t0 <-> t = t0.
-Proof. intuition; inversion H; eauto with imcore. Qed.
-Hint Rewrite invert_term_case_eq : imcore.
-
-Lemma invert_sort_rule_eq c args c' args'
-  : sort_rule c args = sort_rule c' args' <->c = c' /\ args = args'.
-Proof. intuition; try inversion H; subst; eauto  with imcore. Qed.
-Hint Rewrite invert_sort_rule_eq : imcore.
-
-Lemma invert_term_rule_eq c args t c' args' t'
-  : term_rule c args t = term_rule c' args' t' <-> c = c' /\ args = args' /\ t = t'.
-Proof. intuition; try inversion H; subst; eauto  with imcore. Qed.
-Hint Rewrite invert_term_rule_eq : imcore.
-
-(*TODO: move to the right places*)
-Lemma invert_wf_lang_cons l r n
-  : wf_lang ((n,r)::l) <-> fresh n l /\ wf_rule l r /\ wf_lang l.
-Proof.
-  intuition; try inversion H; eauto with imcore.
-Qed.
-Hint Rewrite invert_wf_lang_cons : imcore.
-
-Lemma invert_wf_sort_rule l c args
-  : wf_rule l (sort_rule c args) <-> wf_ctx l c /\ subseq args (map fst c).
-Proof.
-  intuition; try inversion H; eauto with imcore.
-Qed.
-Hint Rewrite invert_wf_sort_rule : imcore.
-
-Lemma invert_wf_term_rule l c args t
-  : wf_rule l (term_rule c args t) <->
-    wf_ctx l c /\ subseq args (map fst c) /\ wf_sort l c t.
-Proof.
-  intuition; try inversion H; eauto with imcore.
-Qed.
-Hint Rewrite invert_wf_term_rule : imcore.
-
-Lemma invert_le_sort_rule l c t1 t2
-  : wf_rule l (sort_le c t1 t2) <->
-    wf_ctx l c /\  wf_sort l c t1 /\ wf_sort l c t2.
-Proof.
-  intuition; try inversion H; eauto with imcore.
-Qed.
-Hint Rewrite invert_le_sort_rule : imcore.
-
-Lemma invert_le_term_rule l c e1 e2 t
-  : wf_rule l (term_le c e1 e2 t) <->
-    wf_ctx l c /\  wf_sort l c t
-    /\ wf_term l c e1 t /\ wf_term l c e2 t.
-Proof.
-  intuition; try inversion H; eauto with imcore.
-Qed.
-Hint Rewrite invert_le_term_rule : imcore.
-
-Lemma wf_args_lang_monotonicity_app l c al args el c' l'
-  : wf_args l c al args el c' -> wf_args (l' ++ l) c al args el c'.
-Proof.
-  induction l'; simpl; intros; break; eauto using wf_args_lang_monotonicity.
-Qed.
-Hint Resolve wf_args_lang_monotonicity_app : imcore.
-
-Lemma le_sort_lang_monotonicity_app l c t1 t2 l'
-  : le_sort l c t1 t2 -> le_sort (l' ++ l) c t1 t2.
-Proof.
-  induction l'; simpl; intros; break; eauto using le_sort_lang_monotonicity.
-Qed.  
-Hint Resolve le_sort_lang_monotonicity_app : imcore.
-
-Lemma term_compiles_to_mono c e t e' src cmp src' cmp'
-  : term_compiles_to src cmp c e t e' ->
-    term_compiles_to (src'++ src) (cmp'++ cmp) c e t e'.
-Proof.
-  induction 1; econstructor; rewrite ?mem_cat;
-    autorewrite with bool_utils in *;
-    eauto with imcore.
-    admit.
-    (*TODO: need stronger IH
-    clear H H0 H1 args t.
-    induction H2; simpl; eauto with imcore.
-    constructor; eauto with imcore.*)
-Admitted.
-
-
-Lemma ctx_compiles_to_mono c c' src cmp src' cmp'
-  : ctx_compiles_to src cmp c c' ->
-    ctx_compiles_to (src'++ src) (cmp'++ cmp) c c'.
-Admitted.
-Hint Resolve ctx_compiles_to_mono : imcore.
-
-
-Lemma term_compiles_to_strengthen tgt src cmp c t e e' src' cmp'
-  : wf_sort src c t ->
-    preserving_compiler tgt src cmp ->
-    term_compiles_to (src'++src) (cmp' ++ cmp) c e t e' ->
-    term_compiles_to src cmp c e t e'.
-Proof.
-  (*
-  intro wfc; revert c'.
-  induction wfc; intro c';
-    let H:=fresh in intro H; inversion H; clear H; subst; constructor; eauto with imcore.*)
-Admitted.
-
-Lemma sort_compiles_to_strengthen tgt src cmp c t t' src' cmp'
-  : wf_sort src c t ->
-    preserving_compiler tgt src cmp ->
-    sort_compiles_to (src'++src) (cmp' ++ cmp) c t t' ->
-    sort_compiles_to src cmp c t t'.
-Proof.
-  (*
-  intro wfc; revert c'.
-  induction wfc; intro c';
-    let H:=fresh in intro H; inversion H; clear H; subst; constructor; eauto with imcore.*)
-Admitted.
-
-Lemma ctx_compiles_to_strengthen tgt src cmp c c' src' cmp'
-  : wf_ctx src c ->
-    preserving_compiler tgt src cmp ->
-    ctx_compiles_to (src'++src) (cmp' ++ cmp) c c' ->
-    ctx_compiles_to src cmp c c'.
-Proof.
-  (*
-  intro wfc; revert c'.
-  induction wfc; intro c';
-    let H:=fresh in intro H; inversion H; clear H; subst; constructor; eauto with imcore.*)
-Admitted.
-
-Ltac solve_inv_lem :=
-  setup_inv_lem;
-  induction 1; [ by compute |..];
-    intros; simpl in *; break;
-      autorewrite with bool_utils imcore in *;
-      intuition; subst;
-        repeat match goal with
-      [H : is_true(in_once _ _ _)|- _] =>
-      rewrite -all_fresh_in_once in H
-      | [ H : ctx_compiles_to (?r::?l) _ _ _|-_] =>
-      change (r::l) with ([::r]++l) in H
-      | [ H : ctx_compiles_to _ (?r::?l) _ _|-_] =>
-      change (r::l) with ([::r]++l) in H
-      | [ H : ctx_compiles_to _ ?cmp _ _|-_] =>
-        is_var cmp; change (cmp) with ([::] ++ cmp) in H
-      | [ H : sort_compiles_to (?r::?l) _ _ _ _|-_] =>
-      change (r::l) with ([::r]++l) in H
-      | [ H : sort_compiles_to _ (?r::?l) _ _ _|-_] =>
-      change (r::l) with ([::r]++l) in H
-      | [ H : sort_compiles_to _ ?cmp _ _ _|-_] =>
-        is_var cmp; change (cmp) with ([::] ++ cmp) in H
-      | [ H : term_compiles_to (?r::?l) _ _ _ _ _|-_] =>
-      change (r::l) with ([::r]++l) in H
-      | [ H : term_compiles_to _ (?r::?l) _ _ _ _|-_] =>
-      change (r::l) with ([::r]++l) in H
-      | [ H : term_compiles_to _ ?cmp _ _ _ _|-_] =>
-        is_var cmp; change (cmp) with ([::] ++ cmp) in H
-    | [H : is_true((?n, _)\in ?cmp),
-       H1 : is_true(fresh ?n ?l),
-            H2 : preserving_compiler _ ?l ?cmp |-_] =>
-      exfalso;
-      let H' := fresh in
-      pose proof (preserving_compiler_fresh H2 H1) as H';
-        let H'' := fresh in
-        pose proof (fresh_neq_in H' H) as H'';
-          move: H'' => /eqP; tauto
-    | [wfl : wf_lang ?l,
-             H : is_true ((_,_)\in ?l) |- _] =>
-      pose proof (rule_in_wf wfl H) as H'; inversion H'; clear H H'; subst
-    end;
-        eauto 7 using sort_compiles_to_strengthen,
-        term_compiles_to_strengthen,
-        ctx_compiles_to_strengthen with imcore.
-
-Lemma preserving_sort_case_inv n t c c' args lt cmp ls
-  :  preserving_compiler lt ls cmp ->
-     wf_lang ls ->
-     (n, sort_rule c args) \in ls ->
-     (n, sort_case t) \in cmp ->
-     ctx_compiles_to ls cmp c c' ->
-     wf_sort lt c' t.
-Proof using .
-  solve_inv_lem.
+  induction 1; 
+    repeat (simpl; autorewrite with bool_utils pfcore utils); eauto with pfcore.
+  all: intuition.
+  all: try match goal with [H : exists _,_|-_] => destruct H end.
+  all: try solve[exists x; 
+    repeat (simpl; autorewrite with bool_utils pfcore utils); by eauto with pfcore].
+  exists eeq;
+    repeat (simpl; autorewrite with bool_utils pfcore utils); by eauto with pfcore.
+  Unshelve.
+  exact (ax "").
 Qed.
 
-Lemma preserving_term_case_inv n e t t' c c' args lt cmp ls
-  :  preserving_compiler lt ls cmp ->
-     wf_lang ls ->
-     (n, term_rule c args t) \in ls ->
-     (n, term_case e) \in cmp ->
-     ctx_compiles_to ls cmp c c' ->
-     sort_compiles_to ls cmp c t t' ->
-     wf_term lt c' e t'.
-Proof using .
-  solve_inv_lem.
-Qed.
-
-
-Lemma preserving_sort_le_inv n t1 t1' t2 t2' c c' lt cmp ls
-  :  preserving_compiler lt ls cmp ->
-     wf_lang ls ->
-     (n, sort_le c t1 t2) \in ls ->
-     ctx_compiles_to ls cmp c c' ->
-     sort_compiles_to ls cmp c t1 t1' ->
-     sort_compiles_to ls cmp c t2 t2' ->
-     le_sort lt c' t1' t2'.
-Proof using . solve_inv_lem. Qed.
-
-
-Lemma preserving_term_le_inv n e1 e1' e2 e2' t t' c c' lt cmp ls
-  :  preserving_compiler lt ls cmp ->
-     wf_lang ls ->
-     (n, term_le c e1 e2 t) \in ls ->
-     ctx_compiles_to ls cmp c c' ->
-     sort_compiles_to ls cmp c t t' ->
-     term_compiles_to ls cmp c e1 t e1' ->
-     term_compiles_to ls cmp c e2 t e2' ->
-     le_term lt c' t' e1' e2'.
-Proof using . solve_inv_lem. Qed.
-
-
-Lemma f_apply_case_map {A B} (f : A -> B) cc b1 b2
-  : f match cc with
-      | sort_case c_case => b1 c_case
-      | term_case c_case => b2 c_case
-      end
-    = match cc with
-      | sort_case c_case => f (b1 c_case)
-      | term_case c_case => f (b2 c_case)
-      end.
-Proof.
-  case: cc; reflexivity.
-Qed.
-
-
-Lemma subst_zip args s s'
-  : (zip args s)[/s'/] = zip args s[/s'/].
-Proof.
-  elim: args s; intros until s; case: s; intros; break; simpl in *; auto.
-  f_equal.
-  by fold_Substable.
-Qed.
-
-
-(* TODO: finish these
-Lemma compile_subst_lookup s n cmp
-  : compile_term cmp (subst_lookup s n) = subst_lookup (compile_subst cmp s) n.
-Proof.
-  elim: s; intros; break; simpl in *; auto.
-  change (?n =? ?s)%string with (n==s).
-  case neq: (n == s); simpl in *; auto.
-Qed.
-
-Lemma compile_term_subst cmp e s
-  : well_scoped (map fst s) e -> compile_term cmp (e[/s/]) = (compile_term cmp e)[/compile_subst cmp s/]
-with compile_args_subst cmp e s
-  : well_scoped (map fst s) e -> compile_args cmp (e[/s/]) = (compile_args cmp e)[/compile_subst cmp s/].
-Proof.
-  {
-    case: e; intros; simpl in *; auto using compile_subst_lookup.
-    case_match; simpl; auto.
-    rewrite subst_assoc; fold_Substable.
-    {
-      rewrite subst_zip.
-      unfold compile_args in *.
-      by rewrite compile_args_subst.
-    }
-    {
-      Search _ (map _ (zip _ _)).
-(* TODO: ws assumption; need ws_compiler
- *)
-Admitted.
-Proof.
-  (* TODO: requires induction *)
-Admitted.
-
-Lemma compile_sort_subst cmp t s
-  : compile_sort cmp (t[/s/]) = (compile_sort cmp t)[/compile_subst cmp s/].
-Proof.
-  case: t; simpl.
-  intros n a.
-  case_match; simpl; auto.
-  rewrite subst_assoc.
-  fold_Substable.
-  rewrite subst_zip.
-  Lemma subst_zip
-    : (zip args s)[/s'/] = zip args s[/s'/].
-  rewrite (f_apply_case_map (sort_subst (compile_subst cmp s))).
-  f_equal_match; simpl; auto.
-Admitted.
-
-
-
-
-Lemma with_names_from_zip c s
-  : with_names_from c s = zip (map fst c) s.
-Proof.
-  elim: c s; [| case]; intros until s; case: s; simpl; auto.
-  intros.
-  f_equal.
-  eauto.
-Qed.
-
-
-Lemma compile_with_names_from cmp c s
-  : compile_subst cmp (with_names_from c s)
-    = with_names_from c (map (compile_term cmp) s).
-Proof.
-  elim: c s; [| case]; intros until s; case: s; simpl; auto.
-  intros.
-  f_equal.
-  eauto.
-Qed.
-
- *)
-
-(*
-(*TODO: not true b/c not a fn!*)
-Lemma compile_ctx_in ls cmp n t t' c c'
-  : ctx_compiles_to ls cmp c c' ->
-    (n,t) \in c ->
-    sort_compiles_to ls cmp t t' ->
-    (n, t') \in c'.
-*)
-
-(*
-Lemma compile_ctx_fst c cmp : map fst (compile_ctx cmp c) = map fst c.
-Proof.
-  elim: c; auto.
-  case => n s l //= -> //.
-Qed.
- *)
-
-Lemma inductive_implies_term_wf lt ls cmp
-  : wf_lang ls -> wf_lang lt -> preserving_compiler lt ls cmp ->
-    term_wf_preserving_sem ls lt cmp
-with inductive_implies_args_wf lt ls cmp
-  : wf_lang ls -> wf_lang lt -> preserving_compiler lt ls cmp ->
-    args_wf_preserving_sem ls lt cmp.
-Proof.
-  all: intros.
-  {
-    unfold term_wf_preserving_sem.
-    intros.
-    destruct H4; simpl.
-    {
-      constructor.
-      (*TODO: not true b/c not a fn!*)
-      Lemma compile_ctx_in
-    revert dependent t'.
-    revert dependent c'.
-    destruct H4
-
-  
 Lemma inductive_implies_semantic ls lt cmp
+  : wf_lang ls -> wf_lang lt -> preserving_compiler lt cmp ls ->
+    semantics_preserving ls lt cmp.
 Proof.
-  intros; unfold semantics_preserving.
-  Scheme sort_wf_ind' := Minimality for wf_sort Sort Prop
-  with term_wf_ind' := Minimality for wf_term Sort Prop
-  with args_wf_ind' := Minimality for wf_args Sort Prop
-  with sort_le_ind' := Minimality for le_sort Sort Prop
-  with term_le_ind' := Minimality for le_term Sort Prop
-    with args_le_ind' := Minimality for le_args Sort Prop.
-  Combined Scheme judge_ind from
-           sort_wf_ind',
-           term_wf_ind',
-           args_wf_ind',
-           sort_le_ind',
-           term_le_ind',
-           args_le_ind'.
-  repeat match goal with [|-context[?f ls lt cmp]] =>
-                         unfold f end.
-  simple apply judge_ind.
-  : 
-     
-
-Lemma inductive_implies_semantic_sort_wf cmp ls lt
-  : wf_lang ls -> wf_lang lt -> preserving_compiler lt cmp ls ->
-    sort_wf_preserving_sem cmp ls lt
-with inductive_implies_semantic_term_wf cmp ls lt
-  : wf_lang ls -> wf_lang lt -> preserving_compiler lt cmp ls ->
-    term_wf_preserving_sem cmp ls lt
-with inductive_implies_semantic_args_wf cmp ls lt
-  : wf_lang ls -> wf_lang lt -> preserving_compiler lt cmp ls ->
-    args_wf_preserving_sem cmp ls lt
-with inductive_implies_semantic_ctx_wf cmp ls lt
-  : wf_lang ls -> wf_lang lt -> preserving_compiler lt cmp ls ->
-    ctx_wf_preserving_sem cmp ls lt
-with inductive_implies_semantic_sort_le cmp ls lt
-  : wf_lang ls -> wf_lang lt -> preserving_compiler lt cmp ls ->
-    sort_le_preserving_sem cmp ls lt
-with inductive_implies_semantic_term_le cmp ls lt
-  : wf_lang ls -> wf_lang lt -> preserving_compiler lt cmp ls ->
-    term_le_preserving_sem cmp ls lt
-with inductive_implies_semantic_args_le cmp ls lt
-  : wf_lang ls -> wf_lang lt -> preserving_compiler lt cmp ls ->
-    args_le_preserving_sem cmp ls lt.
-Proof.
-  all: intros wfs wft pc c.
+  intros; apply judge_ind; intros;
+    repeat (simpl; autorewrite with bool_utils pfcore utils in * ); eauto with pfcore.
   {
-    intros t.    
-    case; intros; simpl.
-    pose in_cmp := i; eapply in_preserving_sort in in_cmp; destruct in_cmp as [e H]; eauto.
-    erewrite named_list_all_fresh_lookup; eauto using preserving_compiler_fresh.
-    simpl.
-    eapply mono_subst_wf_sort; auto. 
-    { eapply preserving_sort_case_inv; eauto. }
-    {
-      eapply inductive_implies_semantic_ctx_wf; [| |eauto |]; eauto with judgment.
-    }
-    {
-      replace (map fst c') with (map fst (compile_ctx cmp c')).
-      apply wf_subst_from_wf_args.
-      eapply inductive_implies_semantic_args_wf;  [| |eauto |]; eauto with judgment.
-      admit(* TODO: lemma*).
-    }
-    {
-      eauto using preserving_compiler_all_fresh, wf_lang_all_fresh.
-    }
+    apply inductive_implies_semantic_sort_axiom; assumption.
   }
   {
-    intros e t.
-    case; intros; simpl.
-    {
-       pose in_cmp := i; eapply in_preserving_term in in_cmp; destruct in_cmp as [e' H]; eauto.
-       erewrite named_list_all_fresh_lookup; eauto using preserving_compiler_fresh.
-       simpl.
-       rewrite compile_sort_subst.
-       rewrite -with_names_from_zip.
-       rewrite -compile_with_names_from.
-       eapply mono_subst_wf_term; eauto. 
-       { admit (*TODO: term version eapply preserving_sort_case_inv; eauto.*). }
-       {
-         eapply inductive_implies_semantic_ctx_wf; [| |eauto |]; eauto.
-         apply rule_in_wf in i; auto.
-         inversion i; subst; eauto.
-       }
-       {
-         admit(*
-         rewrite compile_subst_compile_args.
-         apply wf_subst_from_wf_args.
-         eapply inductive_implies_semantic_args_wf;  [| |eauto |]; eauto with judgment.
-         admitTODO: lemma*).
-       }
-       {
-         eauto using preserving_compiler_all_fresh, wf_lang_all_fresh.
-       }
-    }
-    {
-      eapply wf_term_conv.
-      { eapply inductive_implies_semantic_sort_wf; [| |eauto |]; eauto. }
-      { eapply inductive_implies_semantic_term_wf; [| |eauto |]; eauto. }
-      { eapply inductive_implies_semantic_sort_le; [| |eauto |]; eauto. }
-    }
-    {
-      constructor; eauto.
-      by apply compile_ctx_in.
-    }
+    apply inductive_implies_semantic_term_axiom; assumption.
   }
   {
-    intro_to wf_args; case; simpl; constructor.
-    { by apply fresh_compile_ctx. }
-    { eapply inductive_implies_semantic_args_wf; [| |eauto |]; eauto. }
-    { eapply inductive_implies_semantic_sort_wf; [| |eauto |]; eauto. }
-    {
-      rewrite -compile_with_names_from.
-      rewrite -compile_sort_subst.
-      eapply inductive_implies_semantic_term_wf; [| |eauto |]; eauto.
-      rewrite with_names_from_zip.
-      rewrite compile_ctx_fst.
-      rewrite -with_names_from_zip.
-      done.
-    }
-  }
-  {
-    intro_to wf_ctx; case; simpl; constructor.
-    { by apply fresh_compile_ctx. }
-    { eapply inductive_implies_semantic_ctx_wf; [| |eauto |]; eauto. }
-    { eapply inductive_implies_semantic_sort_wf; [| |eauto |]; eauto. }
-  }
-  {
-    intro_to le_sort; case; simpl; intros.
-    {
-      admit (*TODO: inversion lemma*).
-    }
-    {
-      rewrite !compile_sort_subst.
-      eapply le_sort_subst.
-      { admit (*TODO: le subst,not leargs?
-                eapply inductive_implies_semantic_subst_le; [| |eauto |]; eauto.*). }
-      { eapply inductive_implies_semantic_sort_le; [| |eauto |]; eauto. }
-    }
-    { eapply le_sort_refl. }
-    { eapply le_sort_trans.
-      { eapply inductive_implies_semantic_sort_le; [| |eauto |]; eauto. }
-      { eapply inductive_implies_semantic_sort_le; [| |eauto |]; eauto. }
-    }
-    {
-      eapply le_sort_sym.
-      { eapply inductive_implies_semantic_sort_le; [| |eauto |]; eauto. }
-    }
-  }
-  {
-    intro_to le_term; case; simpl; intros.
-    {
-      rewrite !compile_sort_subst.
-      rewrite !compile_term_subst.
-      eapply le_term_subst.
-      { admit (*TODO: le subst,not leargs?
-                eapply inductive_implies_semantic_subst_le; [| |eauto |]; eauto.*). }
-      { eapply inductive_implies_semantic_term_le; [| |eauto |]; eauto. }
-    }
     
-    {
-      admit (*TODO: inversion lemma*).
-    }
-    { eapply le_term_refl. }
-    { eapply le_term_trans.
-      { eapply inductive_implies_semantic_term_le; [| |eauto |]; eauto. }
-      { eapply inductive_implies_semantic_term_le; [| |eauto |]; eauto. }
-    }
-    {
-      eapply le_term_sym.
-      { eapply inductive_implies_semantic_term_le; [| |eauto |]; eauto. }
-    }
-    {
-      eapply le_term_conv.
-      { eapply inductive_implies_semantic_sort_le; [| |eauto |]; eauto. }
-      { eapply inductive_implies_semantic_term_le; [| |eauto |]; eauto. }
-    }
-  }
-  {
-    intro_to le_args; case; simpl; intros; constructor.
-    { eapply inductive_implies_semantic_args_le; [| |eauto |]; eauto. }
-    { by apply fresh_compile_ctx. }
-    {
-      rewrite -compile_with_names_from.
-      rewrite -compile_sort_subst.
-      eapply inductive_implies_semantic_term_le; [| |eauto |]; eauto.
-      rewrite with_names_from_zip.
-      rewrite compile_ctx_fst.
-      rewrite -with_names_from_zip.
-      done.
-    }
-  }
-Admitted.
-  
-        
     
-
-Lemma inductive_implies_semantic cmp ls lt
-  : wf_lang ls -> wf_lang lt ->
-    preserving_compiler lt cmp ls ->
-    semantics_preserving cmp ls lt.
+    TODO: why is there s and es?
 Proof.
-  intros.
-  repeat split.
-  by eapply inductive_implies_semantic_sort_wf.
-  by eapply inductive_implies_semantic_term_wf.
-  by eapply inductive_implies_semantic_args_wf.
-  by eapply inductive_implies_semantic_sort_le.
-  by eapply inductive_implies_semantic_term_le.
-  by eapply inductive_implies_semantic_args_le.
+  inductive_implies_semantic_rule.
 Qed.
-
-(*
-Lemma semantic_implies_inductive cmp ls lt
-  : wf_lang ls -> wf_lang lt ->
-    semantics_preserving cmp ls lt ->
-    preserving_compiler lt cmp ls.
-Proof.
-  (* TODO: actually quite non-trivial *)
-*)
-*)
-
-*)
-
-(*Note: args not helpful*)
-Fixpoint make_compiler
-           (cmp_sort : string -> list string -> sort)
-           (cmp_exp : string -> list string -> exp)
-           (l : lang) : compiler :=
-  match l with
-  | (n,sort_rule c args)::l' =>
-    (n,sort_case (cmp_sort n (map fst c)))
-      ::(make_compiler cmp_sort cmp_exp l')
-  | (n,term_rule c args _)::l' => (n,term_case (cmp_exp n (map fst c)))
-      ::(make_compiler cmp_sort cmp_exp l')
-  | (n,_)::l' => 
-    (make_compiler cmp_sort cmp_exp l')
-  | [::] => [::]
-  end.
+    TODO: con lemma
+    constructor; eauto.
+    
+    rewrite compile_wfexp_subst in H5.
+    
+    
+    clear H4 H5.
+    match goal with
+    |
+    strategy: separate lemma?
+     -context population tactic for adding e1, e2 wf, etc
+    all: repeat match goal with
+                | [H : wf_ctx _ _ |-_] =>
+                  rewrite (compile_strengthen_ctx _ _ H); eauto with pfcore
+                | [H : wf_sort _ _ _|-_] =>
+                  rewrite (compile_strengthen_sort _ _ H); eauto with pfcore
+                | [H : wf_term _ _ _ _ |-_] =>
+                  rewrite (compile_strengthen_term _ _ H); eauto with pfcore
+                | [H : le_sort _ _ _ _ _|-_] =>
+                  solve[erewrite (compile_strengthen_sort_pf); eauto with pfcore]
+                | [H : eq_term _ _ _ _ _ _ |-_] =>
+                  solve[erewrite (compile_strengthen_term_pf); eauto with pfcore]
+                end.
+ 
+  cbn [compile_pf]; 
+    repeat (simpl; autorewrite with bool_utils pfcore utils).
+  assumption.
+    
+Abort.
