src/named/Core.v
@@ -6,7 +6,7 @@ Import ListNotations.
 Open Scope string.
 Open Scope list.
 From Utils Require Import Utils.
-From Named Require Import Exp ARule.
+From Named Require Export Exp ARule.
 
 (*TODO: why does this generate warnings?*)
 Import Exp.Notations.
@@ -29,102 +29,102 @@ Section TermsAndRules.
     that their sorts are wf.
    *)
   
-  Inductive le_sort : ctx -> sort -> sort -> Prop :=
-  | le_sort_by : forall c name t1 t2,
-      In (name, sort_le c t1 t2) l ->
-      le_sort c t1 t2
-  | le_sort_subst : forall c s1 s2 c' t1' t2',
+  Inductive eq_sort : ctx -> sort -> sort -> Prop :=
+  | eq_sort_by : forall c name t1 t2,
+      In (name, sort_eq_rule c t1 t2) l ->
+      eq_sort c t1 t2
+  | eq_sort_subst : forall c s1 s2 c' t1' t2',
       (* Need to assert wf_ctx c here to satisfy
          assumptions' presuppositions
        *)
       wf_ctx c' ->
-      le_subst c c' s1 s2 ->
-      le_sort c' t1' t2' ->
-      le_sort c t1'[/s1/] t2'[/s2/]
-  | le_sort_con : forall c name c' args s1 s2 es1 es2,
+      eq_subst c c' s1 s2 ->
+      eq_sort c' t1' t2' ->
+      eq_sort c t1'[/s1/] t2'[/s2/]
+  | eq_sort_con : forall c name c' args s1 s2 es1 es2,
       In (name, (sort_rule c' args)) l ->
-      le_args c c' s1 s2 args es1 es2 ->
-      le_sort c (scon name s1) (scon name s2)
-  | le_sort_trans : forall c t1 t12 t2,
-      le_sort c t1 t12 ->
-      le_sort c t12 t2 ->
-      le_sort c t1 t2
-  | le_sort_sym : forall c t1 t2, le_sort c t1 t2 -> le_sort c t2 t1
-  with le_term : ctx -> sort -> exp -> exp -> Prop :=
-  | le_term_subst : forall c s1 s2 c' t e1 e2,
+      eq_args c c' s1 s2 args es1 es2 ->
+      eq_sort c (scon name s1) (scon name s2)
+  | eq_sort_trans : forall c t1 t12 t2,
+      eq_sort c t1 t12 ->
+      eq_sort c t12 t2 ->
+      eq_sort c t1 t2
+  | eq_sort_sym : forall c t1 t2, eq_sort c t1 t2 -> eq_sort c t2 t1
+  with eq_term : ctx -> sort -> exp -> exp -> Prop :=
+  | eq_term_subst : forall c s1 s2 c' t e1 e2,
       (* Need to assert wf_ctx c' here to satisfy
          assumptions' presuppositions
        *)
       wf_ctx c' ->
-      le_subst c c' s1 s2 ->
-      le_term c' t e1 e2 ->
-      le_term c t[/s2/] e1[/s1/] e2[/s2/]
-  | le_term_by : forall c name t e1 e2,
-      In (name,term_le c e1 e2 t) l ->
-      le_term c t e1 e2
-  | le_term_con : forall c name c' args t s1 s2 es1 es2,
+      eq_subst c c' s1 s2 ->
+      eq_term c' t e1 e2 ->
+      eq_term c t[/s2/] e1[/s1/] e2[/s2/]
+  | eq_term_by : forall c name t e1 e2,
+      In (name,term_eq_rule c e1 e2 t) l ->
+      eq_term c t e1 e2
+  | eq_term_con : forall c name c' args t s1 s2 es1 es2,
       In (name, (term_rule c' args t)) l ->
-      le_args c c' s1 s2 args es1 es2 ->
-      le_term c t[/with_names_from c' es2/] (con name s1) (con name s2)
-  | le_term_var : forall c x t,
+      eq_args c c' s1 s2 args es1 es2 ->
+      eq_term c t[/with_names_from c' es2/] (con name s1) (con name s2)
+  | eq_term_var : forall c x t,
       In (x,t) c ->
-      le_term c t (var x) (var x)
-  | le_term_trans : forall c t e1 e12 e2,
-      le_term c t e1 e12 ->
-      le_term c t e12 e2 ->
-      le_term c t e1 e2
-  | le_term_sym : forall c t e1 e2, le_term c t e1 e2 -> le_term c t e2 e1
+      eq_term c t (var x) (var x)
+  | eq_term_trans : forall c t e1 e12 e2,
+      eq_term c t e1 e12 ->
+      eq_term c t e12 e2 ->
+      eq_term c t e1 e2
+  | eq_term_sym : forall c t e1 e2, eq_term c t e1 e2 -> eq_term c t e2 e1
   (* Conversion:
 
 c |- e1 = e2 : t 
                ||
 c |- e1 = e2 : t'
    *)
-  | le_term_conv : forall c t t',
-      le_sort c t t' ->
+  | eq_term_conv : forall c t t',
+      eq_sort c t t' ->
       forall e1 e2,
-        le_term c t e1 e2 ->
-        le_term c t' e1 e2
+        eq_term c t e1 e2 ->
+        eq_term c t' e1 e2
   (* TODO: do I want to allow implicit elements in substitutions? *)
-  (* TODO: do I want to define this in terms of le_args? *)
-  with le_subst : ctx -> ctx -> subst -> subst -> Prop :=
-  | le_subst_nil : forall c, le_subst c [] [] []
-  | le_subst_cons : forall c c' s1 s2,
-      le_subst c c' s1 s2 ->
+  (* TODO: do I want to define this in terms of eq_args? *)
+  with eq_subst : ctx -> ctx -> subst -> subst -> Prop :=
+  | eq_subst_nil : forall c, eq_subst c [] [] []
+  | eq_subst_cons : forall c c' s1 s2,
+      eq_subst c c' s1 s2 ->
       forall name t e1 e2,
         (* assumed because the output ctx is wf: fresh name c' ->*)
-        le_term c t[/s2/] e1 e2 ->
-        le_subst c ((name, t)::c') ((name,e1)::s1) ((name,e2)::s2)
-  with le_args : ctx -> ctx -> list exp -> list exp -> list string -> list exp -> list exp -> Prop :=
-  | le_args_nil : forall c, le_args c [] [] [] [] [] []
-  | le_args_cons_ex : forall c c' s1 s2 args es1 es2,
-      le_args c c' s1 s2 args es1 es2 ->
+        eq_term c t[/s2/] e1 e2 ->
+        eq_subst c ((name, t)::c') ((name,e1)::s1) ((name,e2)::s2)
+  with eq_args : ctx -> ctx -> list exp -> list exp -> list string -> list exp -> list exp -> Prop :=
+  | eq_args_nil : forall c, eq_args c [] [] [] [] [] []
+  | eq_args_cons_ex : forall c c' s1 s2 args es1 es2,
+      eq_args c c' s1 s2 args es1 es2 ->
       forall name t e1 e2,
         (* assumed because the output ctx is wf: fresh name c' ->*)
-        le_term c t[/with_names_from c' es2/] e1 e2 ->
-        le_args c ((name, t)::c') (e1::s1) (e2::s2) (name::args) (e1::es1) (e2::es2)
-  | le_args_cons_im : forall c c' s1 s2 args es1 es2,
-      le_args c c' s1 s2 args es1 es2 ->
+        eq_term c t[/with_names_from c' es2/] e1 e2 ->
+        eq_args c ((name, t)::c') (e1::s1) (e2::s2) (name::args) (e1::es1) (e2::es2)
+  | eq_args_cons_im : forall c c' s1 s2 args es1 es2,
+      eq_args c c' s1 s2 args es1 es2 ->
       forall name t e1 e2,
         (* assumed because the output ctx is wf: fresh name c' ->*)
-        le_term c t[/with_names_from c' es2/] e1 e2 ->
-        le_args c ((name, t)::c') s1 s2 args (e1::es1) (e2::es2)
+        eq_term c t[/with_names_from c' es2/] e1 e2 ->
+        eq_args c ((name, t)::c') s1 s2 args (e1::es1) (e2::es2)
   with wf_term : ctx -> exp -> sort -> Prop :=
   | wf_term_by : forall c n s args c' t,
       In (n, term_rule c' args t) l ->
       wf_args c s c' ->
       wf_term c (con n s) t[/(with_names_from c' s)/]
   | wf_term_conv : forall c e t t',
-      (* We add this condition so that we satisfy the assumptions of le_sort
+      (* We add this condition so that we satisfy the assumptions of eq_sort
          TODO: necessary? not based on current judgment scheme.
          wf_term c e t should imply wf_sort c t,
-         and le_sort c t t' should imply wf_sort c t
+         and eq_sort c t t' should imply wf_sort c t
 
 
       wf_sort c t -> 
        *)
       wf_term c e t ->
-      le_sort c t t' ->
+      eq_sort c t t' ->
       wf_term c e t'
   | wf_term_var : forall c n t,
       In (n, t) c ->
@@ -168,34 +168,52 @@ c |- e1 = e2 : t'
       wf_sort c t ->
       sublist args (map fst c) ->
       wf_rule (term_rule c args t)
-  | le_sort_rule : forall c t1 t2,
+  | eq_sort_rule : forall c t1 t2,
       wf_ctx c ->
       wf_sort c t1 ->
       wf_sort c t2 ->
-      wf_rule (sort_le c t1 t2)
-  | le_term_rule : forall c e1 e2 t,
+      wf_rule (sort_eq_rule c t1 t2)
+  | eq_term_rule : forall c e1 e2 t,
       wf_ctx c ->
       wf_sort c t ->
       wf_term c e1 t ->
       wf_term c e2 t ->
-      wf_rule (term_le c e1 e2 t).
+      wf_rule (term_eq_rule c e1 e2 t).
   
 End TermsAndRules.
-  
-Hint Constructors le_sort le_term le_subst le_args
-     wf_sort wf_term wf_subst wf_args wf_ctx
-     wf_rule : lang_core.
 
-Scheme le_sort_ind' := Minimality for le_sort Sort Prop
-  with le_term_ind' := Minimality for le_term Sort Prop
-  with le_subst_ind' := Minimality for le_subst Sort Prop
+Inductive wf_lang : lang -> Prop :=
+| wf_lang_nil : wf_lang []
+| wf_lang_cons : forall l n r,
+    fresh n l ->
+    wf_lang l ->
+    wf_rule l r ->
+    wf_lang ((n,r)::l).
+  
+Hint Constructors eq_sort eq_term eq_subst eq_args
+     wf_sort wf_term wf_subst wf_args wf_ctx
+     wf_rule wf_lang : lang_core.
+
+Scheme eq_sort_ind' := Minimality for eq_sort Sort Prop
+  with eq_term_ind' := Minimality for eq_term Sort Prop
+  with eq_subst_ind' := Minimality for eq_subst Sort Prop
   with wf_sort_ind' := Minimality for wf_sort Sort Prop
   with wf_term_ind' := Minimality for wf_term Sort Prop
   with wf_args_ind' := Minimality for wf_args Sort Prop
   with wf_ctx_ind' := Minimality for wf_ctx Sort Prop.
 Combined Scheme judge_ind
-         from le_sort_ind', le_term_ind', le_subst_ind',
+         from eq_sort_ind', eq_term_ind', eq_subst_ind',
               wf_sort_ind', wf_term_ind', wf_args_ind',
               wf_ctx_ind'.
 
 (*TODO: separate file for properties?*)
+
+(*Used before a rewrite hint is added to get around
+  the fact that rewrite dbs can't be created
+*)
+Ltac pre_rewrite_core_crush := let x := autorewrite with utils exp in * in
+                                  let y := eauto with utils exp lang_core in
+                                          generic_crush x y.
+Ltac basic_core_crush := let x := autorewrite with utils exp lang_core in * in
+                                  let y := eauto with utils exp lang_core in
+                                          generic_crush x y.
